debias.v
@@ -22,18 +22,18 @@ From zar Require Import
   uniform
 .
 
-Fixpoint debias (t : tree) : tree :=
+Fixpoint debias {A} (t : tree A) : tree A :=
   match t with
   | Leaf x => Leaf x
-  | Fail => Fail
+  | Fail _ => Fail _
   | Choice p f =>
       if Qeq_bool p (1#2) then Choice p (debias ∘ f) else
         tree_bind (bernoulli_tree p)
-          (fun s => if as_bool (s ϵ) then debias (f true) else debias (f false))
+          (fun b => if b then debias (f true) else debias (f false))
   | Fix st G g k => Fix st G (debias ∘ g) (debias ∘ k)
   end.
 
-Lemma wf_tree'_debias (t : tree) :
+Lemma wf_tree'_debias {A} (t : tree A) :
   wf_tree' t ->
   wf_tree' (debias t).
 Proof.
@@ -42,18 +42,18 @@ Proof.
   destruct (Qeq_bool p (1#2)) eqn:Hp.
   - constructor; auto.
   - constructor; eauto with tree.
-    intro s; destruct (as_bool (s ϵ)); auto.
+    intros [|[]]; simpl; auto.
 Qed.
 #[global] Hint Resolve wf_tree'_debias : tree.
 
-Lemma debias_choice q f :
+Lemma debias_choice {A} q (f : bool -> tree A) :
   debias (Choice q f) =
     if Qeq_bool q (1#2) then Choice q (debias ∘ f) else
       tree_bind (bernoulli_tree q)
-        (fun s => if as_bool (s ϵ) then debias (f true) else debias (f false)).
+        (fun b => if b then debias (f true) else debias (f false)).
 Proof. reflexivity. Qed.
 
-Lemma twp_debias t f :
+Lemma twp_debias {A} (t : tree A) f :
   wf_tree' t ->
   twp (debias t) f = twp t f.
 Proof.
@@ -64,17 +64,22 @@ Proof.
       apply Qeq_bool_iff in Hq.
       rewrite Hq.
       unfold compose.
+      rewrite 3!fold_twp.
       rewrite 2!H; auto.
     + rewrite twp_tree_bind_cond; eauto with tree.
+      2: { constructor.
+           - intros _; apply wf_tree_btree_to_tree.
+           - intros []; constructor. }
       rewrite bernoulli_tree_twp_p; try lra; auto.
       rewrite bernoulli_tree_twp_p_compl; try lra; auto.
       rewrite 2!H; auto.
-  - unfold twp; simpl; unfold compose.
+  - existT_inv.
+    unfold twp; simpl; unfold compose.
     f_equal; unfold loop_F.
-    ext k; ext st; destr; auto.
+    ext k; ext st; destr; eauto.
 Qed.
 
-Lemma twlp_debias t f :
+Lemma twlp_debias {A} (t : tree A) f :
   wf_tree' t ->
   bounded f 1 ->
   twlp (debias t) f = twlp t f.
@@ -82,8 +87,11 @@ Proof.
   revert f; induction t; intros f Hwf Hf; inv Hwf; auto.
   - rewrite debias_choice.
     destruct (Qeq_bool q (1#2)) eqn:Hq.
-    + unfold twlp, compose; simpl; rewrite 2!H; auto.
+    + unfold twlp, compose; simpl; rewrite 2!fold_twlp, 2!H; auto.
     + rewrite twlp_tree_bind_cond; eauto with tree.
+      2: { constructor.
+           - intros _; apply wf_tree_btree_to_tree.
+           - intros []; constructor. }
       rewrite bernoulli_tree_twp_p; try lra; auto.
       rewrite bernoulli_tree_twp_p_compl; try lra; auto.
       rewrite 2!H; auto.
@@ -92,17 +100,18 @@ Proof.
            - symmetry; apply twp_strict.
            - intro; eRauto. }
       eRauto.
-  - unfold twlp; simpl; unfold compose.
+  - existT_inv.
+    unfold twlp; simpl; unfold compose.
     unfold dec_iter.
     rewrite 2!inf_apply_eR.
-    f_equal; ext i.
+    f_equal; ext j.
     apply equ_eR.
-    revert s.
+    revert i.
     apply equ_arrow.
     apply equ_f_eR.
-    induction i; simpl; auto.
-    unfold loop_F in *; ext s; destruct (b s); auto.
-    rewrite IHi; apply H; auto.
+    induction j; simpl; auto.
+    unfold loop_F in *; ext s; destruct (b s); eauto.
+    rewrite IHj; apply H; auto.
     intro s'.
     apply leq_eRle.
     revert s'.
@@ -113,7 +122,7 @@ Proof.
         auto; apply wf_tree'_wf_tree; auto.
 Qed.
 
-Theorem tcwp_debias t f :
+Theorem tcwp_debias {A} (t : tree A) f :
   wf_tree' t ->
   tcwp (debias t) f = tcwp t f.
 Proof.
@@ -122,7 +131,7 @@ Proof.
 Qed.
 
 (** De-biasing produces unbiased trees. *)
-Theorem tree_unbiased_debias (t : tree) :
+Theorem tree_unbiased_debias {A} (t : tree A) :
   tree_unbiased (debias t).
 Proof.
   induction t; simpl; try constructor; auto.
@@ -131,14 +140,14 @@ Proof.
     apply Qeq_bool_iff in Hq; auto.
   - constructor.
     + intro s; apply tree_unbiased_btree_to_tree.
-    + intro s; destruct (as_bool (s ϵ)); auto.
+    + intros [|[]]; simpl; auto.
 Qed.
 
 (** Eliminating redundant choices and reducing rationals. *)
-Fixpoint elim_choices (t : tree) : tree :=
+Fixpoint elim_choices {A} (t : tree A) : tree A :=
   match t with
   | Leaf x => Leaf x
-  | Fail => Fail
+  | Fail _ => Fail _
   | Choice p k =>
       if Qeq_bool p 0 then
         elim_choices (k false)
@@ -148,7 +157,7 @@ Fixpoint elim_choices (t : tree) : tree :=
   | Fix st G g k => Fix st G (elim_choices ∘ g) (elim_choices ∘ k)
   end.
 
-Theorem wf_tree'_elim_choices (t : tree) :
+Theorem wf_tree'_elim_choices {A} (t : tree A) :
   wf_tree t ->
   wf_tree' (elim_choices t).
 Proof.
@@ -166,10 +175,10 @@ Proof.
       apply Qred_lt; lra.
     + apply Qred_complete, Qred_correct.
     + intros []; unfold compose; auto.
-  - constructor; eauto.
+  - existT_inv; constructor; eauto.
 Qed.
 
-Lemma twp__elim_choices (fl : bool) (f : St -> eR) (t : tree) :
+Lemma twp__elim_choices {A} (fl : bool) (f : A -> eR) (t : tree A) :
   wf_tree t ->
   twp_ fl (elim_choices t) f = twp_ fl t f.
 Proof.
@@ -189,15 +198,15 @@ Proof.
       * simpl; unfold compose; rewrite 2!H; auto.
         replace (Q2eR (Qred q)) with (Q2eR q); auto.
         rewrite Qred_correct; reflexivity.
-  - f_equal; ext k; ext st; unfold loop_F, compose; destr; auto.
+  - existT_inv; f_equal; ext k; ext st; unfold loop_F, compose; destr; auto.
 Qed.
 
-Corollary twp_elim_choices (f : St -> eR) (t : tree) :
+Corollary twp_elim_choices {A} (f : A -> eR) (t : tree A) :
   wf_tree t ->
   twp (elim_choices t) f = twp t f.
 Proof. apply twp__elim_choices. Qed.
 
-Lemma twlp__elim_choices (fl : bool) (f : St -> eR) (t : tree) :
+Lemma twlp__elim_choices {A} (fl : bool) (f : A -> eR) (t : tree A) :
   wf_tree t ->
   twlp_ fl (elim_choices t) f = twlp_ fl t f.
 Proof.
@@ -217,15 +226,15 @@ Proof.
       * simpl; unfold compose; rewrite 2!H; auto.
         replace (Q2eR (Qred q)) with (Q2eR q); auto.
         rewrite Qred_correct; reflexivity.
-  - f_equal; ext k; ext st; unfold loop_F, compose; destr; auto.
+  - existT_inv; f_equal; ext k; ext st; unfold loop_F, compose; destr; auto.
 Qed.
 
-Corollary twlp_elim_choices (f : St -> eR) (t : tree) :
+Corollary twlp_elim_choices {A} (f : A -> eR) (t : tree A) :
   wf_tree t ->
   twlp (elim_choices t) f = twlp t f.
 Proof. apply twlp__elim_choices. Qed.
 
-Theorem tcwp_elim_choices (f : St -> eR) (t : tree) :
+Theorem tcwp_elim_choices {A} (f : A -> eR) (t : tree A) :
   wf_tree t ->
   tcwp (elim_choices t) f = tcwp t f.
 Proof.
@@ -233,20 +242,20 @@ Proof.
   rewrite twp__elim_choices, twlp__elim_choices; auto.
 Qed.
 
-Inductive reduced : tree -> Prop :=
+Inductive reduced {A} : tree A -> Prop :=
 | reduced_leaf : forall x, reduced (Leaf x)
-| reduced_fail : reduced Fail
+| reduced_fail : reduced (Fail _)
 | reduced_choice : forall q k,
     (0 < q < 1)%Q ->
     Qred q = q ->
     (forall b, reduced (k b)) ->
     reduced (Choice q k)
-| reduce_fix : forall st e g k,
+| reduce_fix : forall I (st : I) e g k,
     (forall s, reduced (g s)) ->
     (forall s, reduced (k s)) ->
     reduced (Fix st e g k).
     
-Theorem reduced_elim_choices (t : tree) :
+Theorem reduced_elim_choices {A} (t : tree A) :
   wf_tree t ->
   reduced (elim_choices t).
 Proof.
@@ -265,25 +274,25 @@ Proof.
         apply Qred_lt; lra.
     + apply Qred_complete, Qred_correct.
     + intro b; apply H; auto.
-  - constructor; eauto.
+  - existT_inv; constructor; eauto.
 Qed.
 
 (** Eliminate fail children of the root. *)
-Fixpoint opt (t : tree) : tree :=
+Fixpoint opt {A} (t : tree A) : tree A :=
   match t with
   | Choice p k =>
       let l := k true in
       let r := k false in
       match (l, r) with
-      | (Fail, _) => opt r
-      | (_, Fail) => opt l
+      | (Fail _, _) => opt r
+      | (_, Fail _) => opt l
       | _ => t
       end
   (* | Fix st e g k => Fix st e (opt ∘ g) k *)
   | _ => t
   end.
 
-Theorem wf_tree_opt (t : tree) :
+Theorem wf_tree_opt {A} (t : tree A) :
   wf_tree t ->
   wf_tree (opt t).
 Proof.
@@ -301,16 +310,17 @@ Proof.
       * constructor; auto.
       * specialize (H true (H3 true)).
         rewrite Ht in H; simpl in H; inv H.
+        existT_inv.
         simpl; constructor; auto.
       * constructor; auto.
       * constructor; auto.
     (* + destruct (t false); constructor; auto. *)
     (*   * specialize (H3 true); rewrite Ht in H3; inv H3; auto. *)
     (*   * specialize (H3 true); rewrite Ht in H3; inv H3; auto. *)
-  - constructor; eauto.
+  - existT_inv; constructor; eauto.
 Qed.
 
-Theorem wf_tree'_opt (t : tree) :
+Theorem wf_tree'_opt {A} (t : tree A) :
   wf_tree' t ->
   wf_tree' (opt t).
 Proof.
@@ -325,12 +335,12 @@ Proof.
       * constructor; auto.
       * constructor; auto.
     + destruct (t false); constructor; auto.
-      * specialize (H5 true); rewrite Ht in H5; inv H5; auto.
-      * specialize (H5 true); rewrite Ht in H5; inv H5; auto.  
-  - constructor; eauto.
+      * specialize (H5 true); rewrite Ht in H5; inv H5; existT_inv; auto.
+      * specialize (H5 true); rewrite Ht in H5; inv H5; existT_inv; auto.
+  - existT_inv; constructor; eauto.
 Qed.
 
-Lemma twp_twlp_opt (f g : St -> eR) (t : tree) :
+Lemma twp_twlp_opt {A} (f g : A -> eR) (t : tree A) :
   wf_tree' t ->
   twp (opt t) f / twlp (opt t) g = twp t f / twlp t g.
 Proof.
@@ -364,7 +374,7 @@ Proof.
       * simpl; rewrite Ht, Hf; reflexivity.
 Qed.
 
-Lemma twlp_opt_pos t f :
+Lemma twlp_opt_pos {A} (t : tree A) f :
   0 < twlp t f ->
   0 < twlp (opt t) f.
 Proof.
@@ -394,11 +404,12 @@ Proof.
     eapply eRmult_eRlt; eauto; eRauto.
 Qed.
 
-Theorem tcwp_opt (f : St -> eR) (t : tree) :
+Theorem tcwp_opt {A} (f : A -> eR) (t : tree A) :
   wf_tree' t ->
   tcwp (opt t) f = tcwp t f.
 Proof.
   intro Ht; unfold tcwp, twp, twlp.
+  rewrite 2!fold_twp, 2!fold_twlp.
   rewrite twp_twlp_opt; auto.
 Qed.
 
@@ -406,7 +417,7 @@ Qed.
 (*                         (fun b => if b then Fail else *)
 (*                                  Choice (1#2) (fun b => if b then Leaf empty else Fail)))). *)
 
-Lemma tree_unbiased_opt (t : tree) :
+Lemma tree_unbiased_opt {A} (t : tree A) :
   tree_unbiased t ->
   tree_unbiased (opt t).
 Proof.
@@ -421,8 +432,5 @@ Proof.
     inv Hub.
     specialize (H true (H3 true)).
     rewrite Ht in H; inv H.
-    simpl.
-    constructor; auto.
-    (* simpl; rewrite <- Ht; inv Hub; auto. *)
-  (* - inv Hub; constructor; eauto. *)
+    existT_inv; simpl; constructor; auto.
 Qed.
