tcwp_facts.v
@@ -6,6 +6,7 @@ From Coq Require Import
   Basics
   QArith
   Reals
+  List
 .
 
 Local Open Scope program_scope.
@@ -24,37 +25,42 @@ From zar Require Import
 
 Local Open Scope eR_scope.
 
-Lemma fold_twp t f :
+Lemma fold_twp {A} (t : tree A) f :
   twp_ false t f = twp t f.
 Proof. reflexivity. Qed.
 
-Lemma twp__bounded (fl : bool) (t : tree) (f : St -> eR) :
+Lemma fold_twlp {A} (t : tree A) f :
+  twlp_ false t f = twlp t f.
+Proof. reflexivity. Qed.
+
+Lemma twp__bounded {A} (fl : bool) (t : tree A) (f : A -> eR) :
   wf_tree t ->
   bounded f 1 ->
   twp_ fl t f <= 1.
 Proof.
   revert f; induction t; simpl; intros f Hwf Hf; inv Hwf; auto.
   - destr; eRauto.
-  -apply eRle_convex_sum; try apply H; eRauto.
+  - apply eRle_convex_sum; try apply H; eRauto.
   - apply leq_eRle.
     unfold iter.
     rewrite sup_apply.
     apply ge_sup.
-    intro i.
-    revert s; apply leq_arrow.
+    intro j.
+    existT_inv.
+    revert i; apply leq_arrow.
     eapply iter_n_bounded.
     { intro; eRauto. }
     intros g Hg s; unfold loop_F; simpl.
     destr; auto.
 Qed.
 
-Corollary twpfail_bounded (t : tree) (f : St -> eR) :
+Corollary twpfail_bounded {A} (t : tree A) (f : A -> eR) :
   wf_tree t ->
   bounded f 1 ->
   twpfail t f <= 1.
 Proof. intros Hwf Hf; apply twp__bounded; auto. Qed.
 
-Lemma twp_bounded (t : tree) (f : St -> eR) (ub : eR) :
+Lemma twp_bounded {A} (t : tree A) (f : A -> eR) (ub : eR) :
   wf_tree t ->
   bounded f ub ->
   twp t f <= ub.
@@ -66,15 +72,17 @@ Proof.
     unfold iter.
     rewrite sup_apply.
     apply ge_sup.
-    intro i.
-    revert s; apply leq_arrow.
+    existT_inv.
+    intro j.
+    revert i; apply leq_arrow.
     eapply iter_n_bounded.
     { intro; eRauto. }
     intros g Hg s; unfold loop_F; simpl.
     destr; auto.
 Qed.
 
-Lemma monotone_twp fl t : monotone (twp_ fl t).
+Lemma monotone_twp {A} fl (t : tree A) :
+  monotone (twp_ fl t).
 Proof.
   induction t; intros f f' Hf; simpl.
   - apply Hf.
@@ -86,7 +94,7 @@ Proof.
     eapply pointwise_le_supremum_le.
     2: { apply sup_spec. }
     2: { apply sup_spec. }
-    intro i; revert s; apply leq_arrow.
+    intro j; revert i; apply leq_arrow.
     apply monotone_iter_n.
     2: { reflexivity. }
     intros g g' Hg.
@@ -96,12 +104,12 @@ Proof.
 Qed.
 #[global] Hint Resolve monotone_twp : twp.
 
-Corollary monotone_twp' fl t :
-  monotone (fun (f0 : St -> eR) (s0 : St) => twp_ fl (t s0) f0).
+Corollary monotone_twp' {A B} fl (t : A -> tree B) :
+  monotone (fun (f0 : B -> eR) (s0 : A) => twp_ fl (t s0) f0).
 Proof. intros f f' Hf s; apply monotone_twp; auto. Qed.
 #[global] Hint Resolve monotone_twp' : twp.
 
-Lemma twp_strict t :
+Lemma twp_strict {A} (t : tree A) :
   twp_ false t (const 0) = 0.
 Proof.
   unfold const; induction t; simpl; try reflexivity.
@@ -109,14 +117,14 @@ Proof.
   - unfold iter, loop_F.
     apply equ_eR; rewrite sup_apply.
     apply supremum_sup, const_supremum.
-    intro i; apply equ_eR.
-    replace 0 with (const 0 s) by reflexivity.
+    intro j; apply equ_eR.
+    replace 0 with (const 0 i) by reflexivity.
     apply f_eq'. unfold const.
-    induction i; simpl; try reflexivity.
-    ext st; destruct (b st); auto; rewrite IHi; apply H.
+    induction j; simpl; try reflexivity.
+    ext st; destruct (b st); auto; rewrite IHj; apply H.
 Qed.
 
-Lemma twp__tree_bind fl t k f :
+Lemma twp__tree_bind {A B} fl (t : tree A) (k : A -> tree B) f :
   twp_ fl (tree_bind t k) f = twp_ fl t (fun s => twp_ fl (k s) f).
 Proof.
   revert k f; induction t; intros k f; simpl; auto.
@@ -124,11 +132,11 @@ Proof.
   - repeat f_equal; ext s'; auto.
 Qed.
 
-Corollary twp_tree_bind t k f :
+Corollary twp_tree_bind {A B} (t : tree A) (k : A -> tree B) f :
   twp (tree_bind t k) f = twp t (fun s => twp (k s) f).
 Proof. apply twp__tree_bind. Qed.
 
-Lemma twlp__tree_bind fl t k f :
+Lemma twlp__tree_bind {A B} fl (t : tree A) (k : A -> tree B) f :
   twlp_ fl (tree_bind t k) f = twlp_ fl t (fun s => twlp_ fl (k s) f).
 Proof.
   revert k f; induction t; intros k f; simpl; auto.
@@ -136,11 +144,11 @@ Proof.
   - repeat f_equal; ext s'; auto.
 Qed.
 
-Corollary twlp_tree_bind t k f :
+Corollary twlp_tree_bind {A B} (t : tree A) (k : A -> tree B) f :
   twlp (tree_bind t k) f = twlp t (fun s => twlp (k s) f).
 Proof. apply twlp__tree_bind. Qed.
 
-Lemma twp_scalar t f c :
+Lemma twp_scalar {A} (t : tree A) f c :
   twp t (fun x => c * f x) = c * twp t f.
 Proof.
   unfold twp; revert f c; induction t; intros f c; simpl; eRauto.
@@ -152,15 +160,15 @@ Proof.
   - unfold iter.
     rewrite 2!sup_apply_eR.
     rewrite sup_scalar.
-    f_equal; ext i.
-    revert s f c.
-    induction i; simpl; intros s f c; unfold const; eRauto.
+    f_equal; ext j.
+    revert i f c.
+    induction j; simpl; intros s f c; unfold const; eRauto.
     unfold loop_F.
     destruct (b s); eRauto.
-    rewrite <- H; f_equal; ext st; apply IHi.
+    rewrite <- H; f_equal; ext st; apply IHj.
 Qed.
 
-Lemma monotone_twlp fl t : monotone (twlp_ fl t).
+Lemma monotone_twlp {A} fl (t : tree A) : monotone (twlp_ fl t).
 Proof.
   induction t; intros f f' Hf; simpl.
   - apply Hf.
@@ -172,7 +180,7 @@ Proof.
     eapply pointwise_le_infimum_le.
     2: { apply inf_spec. }
     2: { apply inf_spec. }
-    intro i; revert s; apply leq_arrow.
+    intro j; revert i; apply leq_arrow.
     apply monotone_iter_n.
     2: { reflexivity. }
     intros g g' Hg.
@@ -182,12 +190,12 @@ Proof.
 Qed.
 #[global] Hint Resolve monotone_twlp : twp.
 
-Corollary monotone_twlp' fl t :
-  monotone (fun (f0 : St -> eR) (s0 : St) => twlp_ fl (t s0) f0).
+Corollary monotone_twlp' {A B} fl (t : A -> tree B) :
+  monotone (fun (f0 : B -> eR) (s0 : A) => twlp_ fl (t s0) f0).
 Proof. intros f f' Hf s; apply monotone_twlp; auto. Qed.
 #[global] Hint Resolve monotone_twlp' : twp.
 
-Lemma twlp_bounded (fl : bool) (t : tree) (f : St -> eR) :
+Lemma twlp_bounded {A} (fl : bool) (t : tree A) (f : A -> eR) :
   wf_tree t ->
   bounded f 1 ->
   twlp_ fl t f <= 1.
@@ -196,7 +204,8 @@ Proof.
   - destruct fl; eRauto.
   - apply eRle_convex_sum; eauto.
     apply Q2eR_le_1; apply H2.
-  - unfold dec_iter.
+  - existT_inv.
+    unfold dec_iter.
     apply leq_eRle.
     rewrite inf_apply.
     apply ge_dinf with O.
@@ -206,7 +215,7 @@ Proof.
       * intro st; apply H; auto.
         intro; reflexivity.
       * intros g g' Hg st; apply monotone_twlp; auto.
-    + revert s; apply leq_arrow.
+    + revert i; apply leq_arrow.
       apply iter_n_bounded.
       * eRauto.
       * intros g Hg s; unfold loop_F; destruct (b s).
@@ -214,7 +223,7 @@ Proof.
         { apply H0; auto. }
 Qed.
 
-Lemma twp__sum fl (t : tree) (f g : St -> eR) :
+Lemma twp__plus {A} fl (t : tree A) (f g : A -> eR) :
   twp_ fl t (fun s => f s + g s) = twp_ false t f + twp_ fl t g.
 Proof.
   unfold twp; revert f g; induction t; intros f g; simpl; auto.
@@ -226,29 +235,29 @@ Proof.
     rewrite <- sup_sum.
     2: { apply chain_iter_n''; auto with twp; intro; eRauto. }
     2: { apply chain_iter_n''; auto with twp; intro; eRauto. }
-    f_equal; ext i.
+    f_equal; ext j.
     apply equ_eR.
-    revert s. apply equ_arrow.
+    revert i. apply equ_arrow.
     apply equ_f_eR.
-    induction i; simpl.
+    induction j; simpl.
     { ext s; eRauto. }
     ext s.
     unfold loop_F; simpl.
     destruct (b s) eqn:Hbs.
-    + unfold loop_F in IHi; rewrite IHi; apply H.
+    + unfold loop_F in IHj; rewrite IHj; apply H.
     + apply H0.
 Qed.
 
-Corollary twp_sum (t : tree) (f g : St -> eR) :
+Corollary twp_plus {A} (t : tree A) (f g : A -> eR) :
   twp t (fun s => f s + g s) = twp t f + twp t g.
-Proof. apply twp__sum. Qed.
+Proof. apply twp__plus. Qed.
 
-Corollary twpfail_sum (t : tree) (f g : St -> eR) :
+Corollary twpfail_plus {A} (t : tree A) (f g : A -> eR) :
   twpfail t (fun s => f s + g s) = twp t f + twpfail t g.
-Proof. apply twp__sum. Qed.
+Proof. apply twp__plus. Qed.
 
 (** [twp_ b c f = 1 - twlp_ (~ b) c (1 - f)] *)
-Theorem twp_twlp_sum (fl : bool) (t : tree) (f : St -> eR) :
+Theorem twp_twlp_sum {A} (fl : bool) (t : tree A) (f : A -> eR) :
   wf_tree t ->
   bounded f 1 ->
   twp_ fl t f + twlp_ (negb fl) t (fun s => 1 - f s) = 1.
@@ -259,7 +268,8 @@ Proof.
   - rewrite <- eRplus_assoc, eRplus_comm4.
     rewrite eRplus_assoc, <- 2!eRmult_plus_distr_l.
     rewrite 2!H; eRauto.
-  - unfold iter, dec_iter.
+  - existT_inv.
+    unfold iter, dec_iter.
     rewrite sup_apply_eR, inf_apply_eR.
     eapply supremum_infimum_sum with (ub:=1%R).
     6: { apply sup_spec. }
@@ -267,28 +277,28 @@ Proof.
     { apply chain_iter_n''; auto with twp; intro; eRauto. }
     { apply dec_chain_iter_n''; auto with twp;
         intro st; apply twlp_bounded; auto; intro; eRauto. }
-    { intro i; revert s; apply leq_arrow; apply iter_n_bounded.
+    { intro j; revert i; apply leq_arrow; apply iter_n_bounded.
       - intro; eRauto.
       - intros g Hg s; unfold loop_F; destr; apply twp__bounded; auto. }
-    { intro i; revert s; apply leq_arrow; apply iter_n_bounded.
+    { intro j; revert i; apply leq_arrow; apply iter_n_bounded.
       - intro; eRauto.
       - intros g Hg s; unfold loop_F; destr;
           apply twlp_bounded; auto; intro; eRauto. }
-    intro i; simpl.
-    revert s.
-    induction i; intro s; simpl.
+    intro j; simpl.
+    revert i.
+    induction j; intro s; simpl.
     { eRauto. }
     unfold loop_F in *.
     destr.
     + replace (iter_n
-                 (fun (k : St -> eR) (s0 : St) =>
+                 (fun (k : I -> eR) (s0 : I) =>
                     if b s0
                     then twlp_ (negb fl) (t s0) k
-                    else twlp_ (negb fl) (t0 s0) (fun s1 : St => 1 - f s1))
-                 (const 1) i) with
-        (fun s => 1 - iter_n (fun (k : St -> eR) (s : St) =>
+                    else twlp_ (negb fl) (t0 s0) (fun s1 : A => 1 - f s1))
+                 (const 1) j) with
+        (fun s => 1 - iter_n (fun (k : I -> eR) (s : I) =>
                              if b s then twp_ fl (t s) k else twp_ fl (t0 s) f)
-                     (const 0) i s).
+                     (const 0) j s).
       2: { ext st; symmetry; apply eRplus_eq_minus; try apply IHi; eRauto. }
       apply H; auto.
       intro s'; apply leq_eRle; revert s'.
@@ -299,7 +309,7 @@ Proof.
 Qed.
 
 (** [twlp b c f = 1 - twp (~ b) c (1 - f)] *)
-Corollary twlp_twp_sum (fl : bool) (t : tree) (f : St -> eR) :
+Corollary twlp_twp_sum {A} (fl : bool) (t : tree A) (f : A -> eR) :
   wf_tree t ->
   bounded f 1 ->
   twlp_ fl t f + twp_ (negb fl) t (fun s => 1 - f s) = 1.
@@ -315,7 +325,7 @@ Proof.
   intro s; eRauto.
 Qed.
 
-Corollary twlp_twp_complement (fl : bool) (t : tree) (f : St -> eR) :
+Corollary twlp_twp_complement {A} (fl : bool) (t : tree A) (f : A -> eR) :
   wf_tree t ->
   bounded f 1 ->
   twlp_ fl t f = 1 - twp_ (negb fl) t (fun s => 1 - f s).
@@ -325,33 +335,34 @@ Proof.
   rewrite eRplus_comm; apply twlp_twp_sum; auto.
 Qed.
 
-Corollary twlp_twpfail_complement (t : tree) (f : St -> eR) :
+Corollary twlp_twpfail_complement {A} (t : tree A) (f : A -> eR) :
   wf_tree t ->
   bounded f 1 ->
   twlp t f = 1 - twpfail t (fun s => 1 - f s).
 Proof. intros Hwf Hf; apply twlp_twp_complement; auto. Qed.
 
-Lemma no_fail'_twp fl t f :
+Lemma no_fail'_twp {A} fl (t : tree A) f :
   no_fail' t ->
   twp_ fl t f = twp t f.
 Proof.
   unfold twp; revert fl f; induction t; intros fl f Ht; inv Ht; simpl; auto.
   - rewrite H; auto; f_equal; f_equal; apply H; auto.
-  - f_equal; unfold loop_F.
+  - existT_inv; f_equal; unfold loop_F.
     ext k; ext st; destruct (b st) eqn:Hbst; auto.
 Qed.
 
-Lemma no_fail'_twlp fl t f :
+Lemma no_fail'_twlp {A} fl (t : tree A) f :
   no_fail' t ->
   twlp_ fl t f = twlp t f.
 Proof.
   unfold twlp; revert fl f; induction t; intros fl f Ht; inv Ht; simpl; auto.
   - rewrite H; auto; f_equal; f_equal; apply H; auto.
-  - f_equal; unfold loop_F.
+  - existT_inv; f_equal; unfold loop_F.
     ext k; ext st; destruct (b st) eqn:Hbst; auto.
 Qed.
 
-Lemma twp_tree_bind_cond (t t1 t2 : tree) (e : St -> bool) (f : St -> eR) :
+Lemma twp_tree_bind_cond {A B}
+  (t : tree A) (t1 t2 : tree B) (e : A -> bool) (f : B -> eR) :
   wf_tree t ->
   wf_tree t1 ->
   wf_tree t2 ->
@@ -363,11 +374,11 @@ Proof.
   rewrite twp_tree_bind.
   rewrite eRmult_comm, <- twp_scalar.
   rewrite eRmult_comm, <- twp_scalar.
-  rewrite <- twp_sum.
+  rewrite <- twp_plus.
   f_equal; ext s; destr; eRauto.
 Qed.
 
-Lemma twp_twlp (t : tree) (f : St -> eR) :
+Lemma twp_twlp {A} (t : tree A) (f : A -> eR) :
   wf_tree t ->
   bounded f 1 ->
   twlp t f = twp t f + twlp t (const 0).
@@ -379,7 +390,7 @@ Proof.
       1 + twpfail t (const 1) = twp t f + 1 + twpfail t (1 - f)
    *)  
   intros Hwf Hf.
-  rewrite (@twlp_twpfail_complement t (const 0)); auto.
+  rewrite (@twlp_twpfail_complement _ t (const 0)); auto.
   2: { intro; eRauto. }
   rewrite eRplus_minus_assoc.
   2: { eRauto. }
@@ -400,7 +411,7 @@ Proof.
   apply eRplus_eq_minus.
   { unfold eRplus; simpl.
     destruct (twpfail t (fun s => 1 - const 0 s)) eqn:Ht; try congruence.
-    assert (Hb: bounded (fun s => 1 - @const eR St 0 s) 1).
+    assert (Hb: bounded (fun s => 1 - @const eR A 0 s) 1).
     { intro; eRauto. }
     eapply twpfail_bounded in Hb; eauto.
     eapply eRle_infty_not_infty in Hb; try congruence.
@@ -409,12 +420,12 @@ Proof.
   rewrite <- eRplus_assoc.
   f_equal.
   rewrite eRplus_comm.
-  rewrite <- twpfail_sum.
+  rewrite <- twpfail_plus.
   f_equal.
   ext s; eRauto.
 Qed.
 
-Lemma twlp_tree_bind_cond (t t1 t2 : tree) (e : St -> bool) (f : St -> eR) :
+Lemma twlp_tree_bind_cond {A B} (t : tree A) (t1 t2 : tree B) (e : A -> bool) (f : B -> eR) :
   wf_tree t ->
   wf_tree t1 ->
   wf_tree t2 ->
@@ -428,19 +439,19 @@ Proof.
   rewrite twlp_tree_bind.
   rewrite eRmult_comm, <- twp_scalar.
   rewrite eRmult_comm, <- twp_scalar.
-  rewrite <- twp_sum.
-  replace (fun s : St => twlp t1 f * (if e s then 1 else 0) +
-                        twlp t2 f * (if e s then 0 else 1)) with
+  rewrite <- twp_plus.
+  replace (fun s : A => twlp t1 f * (if e s then 1 else 0) +
+                       twlp t2 f * (if e s then 0 else 1)) with
     (fun s => if e s then twlp t1 f else twlp t2 f).
   2: { ext s; destr; eRauto. }
-  replace (fun s : St => twlp (if e s then t1 else t2) f) with
-    (fun s : St => if e s then twlp t1 f else twlp t2 f).
+  replace (fun s : A => twlp (if e s then t1 else t2) f) with
+    (fun s : A => if e s then twlp t1 f else twlp t2 f).
   2: { ext s; destr; reflexivity. }
   apply twp_twlp; auto.
   intro s; destr; apply twlp_bounded; auto.
 Qed.
 
-Lemma simple_twp_twlp (f : St -> eR) (t : tree) :
+Lemma simple_twp_twlp {A} (f : A -> eR) (t : tree A) :
   simple t ->
   bounded f 1 ->
   twp t f = twlp t f.
@@ -450,7 +461,7 @@ Proof.
   rewrite 2!H; auto.
 Qed.
 
-Lemma twlp_fail t :
+Lemma twlp_fail {A} (t : tree A) :
   wf_tree t ->
   twlp t (const 1) = 1 - tfail t.
 Proof.
@@ -465,4 +476,23 @@ Proof.
   { apply twlp_twp_sum; auto.
     intro s; eRauto. }
   f_equal; ext s; eRauto.
+Qed.
+
+Lemma tree_all_twp_0 {A} (f : A -> eR) t :
+  simple t ->
+  tree_all (fun s => f s = 0) t ->
+  twp t f = 0.
+Proof.
+  unfold twp.
+  revert f; induction t; simpl; intros f Ht Hall; inv Ht; inv Hall; auto.
+  rewrite 2!H; eRauto.
+Qed.
+
+Lemma twp_sum {A} (t : tree A) (l : list (A -> eR)) :
+  twp_ false t (fun s => sum (map (fun f => f s) l)) = sum (map (fun f => twp t f) l).
+Proof.
+  unfold twp, sum.
+  revert t; induction l; intros t; simpl.
+  - apply twp_strict.
+  - rewrite twp__plus; f_equal; auto.
 Qed.
