tcwp_geometric.v
@@ -20,10 +20,11 @@ From zar Require Import
 
 Local Open Scope order_scope.
 
-Lemma loop_approx''_twp_fix_approx'''
-  (st : St) (e : St -> bool) (g : St -> tree) (k : St -> tree) (n : nat) f :
-  loop_approx'' e (fun f0 s => twp (g s) f0) (fun s => twp (k s) f) n st =
-    twp (fix_approx''' st e g (fun s => if e s then Fail else k s) n) f.
+Lemma loop_approx''_twp_fix_approx''' {I A}
+  (st : I) (e : I -> bool) (g : I -> tree I) (k : I -> tree A) (n : nat) f :
+  loop_approx'' e (fun f0 s => twp_ false (g s) f0)
+    (fun s => twp_ false (k s) f) n st =
+    twp (fix_approx''' st e g (fun s => if e s then Fail _ else k s) n) f.
 Proof.
   unfold twp; revert st e g k f; induction n; intros st e g k f; simpl.
   { unfold loop_approx''; simpl; destr; auto. }
@@ -32,7 +33,7 @@ Proof.
   rewrite twp__tree_bind; f_equal; ext s; apply IHn.
 Qed.
 
-Lemma loop_approx''_false e g f n s :
+Lemma loop_approx''_false {A} e g f n (s : A) :
   e s = false ->
   loop_approx'' e g f n s = f s.
 Proof.
@@ -42,7 +43,7 @@ Proof.
   - unfold loop_F. rewrite Hes; reflexivity.
 Qed.
 
-Lemma g_loop_approx'_loop_approx'' e g f n s :
+Lemma g_loop_approx'_loop_approx'' {A} (e : A -> bool) g f n s :
   e s = true ->
   g (const 0) = const 0 ->
   g (loop_approx' e g f n) s = loop_approx'' e g f n s.
@@ -59,7 +60,7 @@ Proof.
   - symmetry; apply loop_approx''_false; auto.
 Qed.
 
-Lemma shift_loop_approx'_loop_approx'' e g f  :
+Lemma shift_loop_approx'_loop_approx'' {A} (e : A -> bool) g f  :
   g (const 0) = const 0 ->
   shift (loop_approx' e g f) = loop_approx'' e g f.
 Proof.
@@ -72,58 +73,61 @@ Proof.
   - symmetry; apply loop_approx''_false; auto.
 Qed.
 
-Lemma twp_fix_chain_scalar G st a t i :
+Lemma twp_fix_chain_scalar {I} G (st : I) a t i :
   G st = true ->
   twp (fix_chain st G (fun _ => t) i) (fun s => if G s then a else 0) =
-    a *  twp t (fun s : St => if G s then 1 else 0) ^ i.
+    a *  twp t (fun s : I => if G s then 1 else 0) ^ i.
 Proof.
   unfold twp; revert G st a t; induction i; intros G st a t HGst; simpl.
   { rewrite HGst; eRauto. }
   rewrite twp__tree_bind.
-  replace (fun s => twp_ false (if G s then t else Leaf s)
-                   (fun s0 => if G s0 then a else 0)) with
-    (fun s => if G s then twp t (fun s0 : St => if G s0 then a else 0)
-           else 0).
+  replace (fun s : I => twp_ false (if G s then t else Leaf s)
+                       (fun s0 : I => if G s0 then a else 0)) with
+    (fun s : I => if G s then twp t (fun s0 : I => if G s0 then a else 0)
+               else 0).
   2: { ext s; destruct (G s) eqn:HGs; simpl; auto.
        rewrite HGs; reflexivity. }
   rewrite eRmult_comm.
   rewrite eRmult_assoc.
   rewrite (@eRmult_comm _ a).
   erewrite <- IHi; eauto; clear IHi.
-  replace (fun s : St => if G s then a else 0) with
-    (fun s : St => a * (if G s then 1 else 0)).
+  replace (fun s : I => if G s then a else 0) with
+    (fun s : I => a * (if G s then 1 else 0)).
   2: { ext s; destr; eRauto. }
+  rewrite 3!fold_twp.
   rewrite <- twp_scalar; unfold twp.
   f_equal; ext s; destr.
   - eRauto; rewrite eRmult_comm; apply twp_scalar.
   - eRauto.
 Qed.
 
-Lemma twp_fix_chain_geometric_series st G t i f :
+Lemma twp_fix_chain_geometric_series {I} (st : I) G t i f :
   G st = true ->
-  twp (fix_chain st G (fun _ => t) i) (fun s => if G s then 0 else f s) =
+  twp_ false (fix_chain st G (fun _ => t) i) (fun s => if G s then 0 else f s) =
     geometric_series (twp t (fun s => if G s then 0 else f s))
-      (twp t (fun s : St => if G s then 1 else 0)) i.
+      (twp t (fun s : I => if G s then 1 else 0)) i.
 Proof.
   unfold twp; revert st G t f; induction i; intros st G t f HGst; simpl.
   { rewrite HGst; reflexivity. }
   rewrite twp__tree_bind.
   erewrite <- IHi; eauto; clear IHi.
-  replace (fun s : St => twp_ false (if G s then t else Leaf s)
-                        (fun s0 : St => if G s0 then 0 else f s0)) with
-    (fun s => if G s then twp t (fun s0 : St => if G s0 then 0 else f s0) else f s).
+  replace (fun s : I => twp_ false (if G s then t else Leaf s)
+                       (fun s0 : I => if G s0 then 0 else f s0)) with
+    (fun s => if G s then twp t (fun s0 : I => if G s0 then 0 else f s0) else f s).
   2: { ext s; destruct (G s) eqn:HGs; simpl; auto; rewrite HGs; reflexivity. }
   replace (fun s => if G s then twp t (fun s0 => if G s0 then 0 else f s0) else f s)
     with (fun s => (if G s then twp t (fun s0 => if G s0 then 0 else f s0) else 0) +
                   (if G s then 0 else f s)).
   2: { ext s; destr; eRauto. }
-  rewrite twp_sum.
+  rewrite 4!fold_twp.
+  rewrite twp_plus.
   unfold twp.
   rewrite eRplus_comm; f_equal.
+  rewrite 3!fold_twp.
   rewrite twp_fix_chain_scalar; auto.
 Qed.
 
-Lemma twp_fix_iid st (G : St -> bool) t k f :
+Lemma twp_fix_iid {A B} (st : A) (G : A -> bool) (t : tree A) (k : A -> tree B) f :
   wf_tree t ->
   (forall s, wf_tree (k s)) ->
   twp t (fun s => if G s then 1 else 0) < 1 ->
@@ -144,17 +148,17 @@ Proof.
   rewrite loop_approx_loop_approx'.
   replace (shift
              (fun i0 : nat =>
-                loop_approx' G (fun (f0 : St -> eR) (s : St) => twp_ false t f0)
-                  (fun s : St => twp_ false (k s) f) i0 st) i) with
-    (loop_approx'' G (fun (f0 : St -> eR) (s : St) => twp_ false t f0)
-       (fun s : St => twp_ false (k s) f) i st).
+                loop_approx' G (fun (f0 : A -> eR) (s : A) => twp_ false t f0)
+                  (fun s : A => twp_ false (k s) f) i0 st) i) with
+    (loop_approx'' G (fun (f0 : A -> eR) (s : A) => twp_ false t f0)
+       (fun s : A => twp_ false (k s) f) i st).
   2: { rewrite <- shift_loop_approx'_loop_approx''.
        - reflexivity.
        - ext s; apply twp_strict. }
   rewrite loop_approx''_twp_fix_approx'''.
   rewrite fix_approx'''_tree_bind_fix_approx.
   rewrite twp_tree_bind.
-  replace (fun s : St => twp (if G s then Fail else k s) f) with
+  replace (fun s : A => twp (if G s then Fail _ else k s) f) with
     (fun s => if G s then 0 else twp (k s) f).
   2: { ext s; destr; reflexivity. }
   unfold twp.
